src/opt/SplitAcqRel.v
@@ -103,7 +103,7 @@ Proof.
   assert (RELT_LE:
    View.opt_le
      (TView.write_released lc1_src.(Local.tview) sc1_src loc to releasedm_src ord_src)
-     (TView.write_released lc1_tgt.(Local.tview) sc1_tgt loc to releasedm_tgt ord_tgt)).
+     (TView.write_released lc1_tgt.(Local.tview) sc2_tgt loc to releasedm_tgt ord_tgt)).
   { unfold TView.write_released, TView.write_tview. ss. viewtac.
     repeat (condtac; aggrtac;
             try match goal with
@@ -130,8 +130,6 @@ Proof.
     + inv WRITABLE. econs.
       * eapply TimeFacts.le_lt_lt; [apply ACQUIRED1|]. viewtac.
         eapply TimeFacts.le_lt_lt; eauto.
-      * by destruct ord_src, ord_tgt.
-      * by destruct ord_src, ord_tgt.
   - econs; eauto. s.
     unfold TView.write_tview, TView.write_fence_tview, TView.read_fence_tview. ss.
     econs; ss; repeat (condtac; aggrtac).
@@ -146,7 +144,7 @@ Proof.
       etrans; [apply WF1_TGT|]. etrans; [apply WF1_TGT|]. aggrtac.
     + etrans; [apply LOCAL1|]. ss. condtac; aggrtac.
     + etrans; [apply LOCAL1|]. aggrtac.
-  - apply TViewFacts.write_sc_mon; auto.
+  - ss.
 Qed.
 
 Lemma sim_local_write_acqrel
